For the output feedback controller the closed-loop system is given as
\begin{equation}
\begin{split}
    \lambda I-(A+kBC)&=0\\
    \lambda I-A-kBC&=0\\
    (\lambda I-A)X_1n_1-kBCX_1n_1&=0\\
    (\lambda I-A)X_1n_1+BCY_1n_1&=0\\
    \begin{bmatrix}\lambda I-A& BC\end{bmatrix}\begin{bmatrix}X_1n_1\\Y_1n_1\end{bmatrix}&=0\\
\end{split}
\end{equation}
Lets assume $\lambda$ is unknown, then 
\begin{equation}
    \begin{split}
        X_1n_1&=R_{des}(1)\\
        n_1&=X_1^{-1}R_{des}(1)
    \end{split}
\end{equation}
and 
\begin{equation}
\begin{split}
    (\lambda I-A)X_1=\gamma X_1\\
    (\lambda I-\gamma I-A)X_1=0
\end{split}
\end{equation}

