\section{State Feedback Case}
The eigenvalue equation is given as
\begin{equation}
    (A-BK)V=\lambda V
\end{equation}
or 
\begin{equation}
\begin{split}
    \lambda V-(A+BK)V&=0\\
    \lambda V-AV-BKV&=0\\
    (\lambda I-A)X+BY&=0\\
    \begin{bmatrix}
        \lambda I-A& B
    \end{bmatrix}\begin{bmatrix}
        X\\Y
    \end{bmatrix}=0
\end{split}
\end{equation}
where $K=-YX^{-1}$.

\section{Output Feedback Case}
Let $k\in\mathbb{R}$, then
\begin{equation}
\begin{split}
    -YX^{-1}&=kC\\
    -Y&=kCX\\
    kCX+Y&=0\\
    \begin{bmatrix}
        kC&I
    \end{bmatrix}\begin{bmatrix}
        X\\Y
    \end{bmatrix}&=0
\end{split}
\end{equation}
or even 
\begin{equation}
    \begin{split}
        \begin{bmatrix}
            C&I
        \end{bmatrix}\begin{bmatrix}
            kX\\Y
        \end{bmatrix}&=0
    \end{split}
\end{equation}
Using the following 
\begin{equation}
    \begin{bmatrix}
        \lambda_1 I-A& B
    \end{bmatrix}\begin{bmatrix}
        X_1n_1\\Y_1n_1
    \end{bmatrix}=0
\end{equation}
the following needs to be satisfied
\begin{equation}
    \begin{bmatrix}
        C& I
    \end{bmatrix}\begin{bmatrix}
        kX_1n_1\\Y_1n_1
    \end{bmatrix}=0
\end{equation}

